Add pchor version of theorems in endpointCong

projection/proofs/endpointCongScript.sml
@@ -1,24 +1,39 @@
-open preamble endpointLangTheory chor_to_endpointTheory
-              endpointSemTheory  endpointPropsTheory
-              chorSemTheory;
+open preamble endpointLangTheory
+     chor_to_endpointTheory pchor_to_endpointTheory
+     endpointSemTheory  endpointPropsTheory
+     chorSemTheory pchorSemTheory
 
 val _ = new_theory"endpointCong"
 
 (* Given a network, returns all the process identifiers
    (note it can give duplicated results
 *)
-val network_procs_def = Define`
+Definition network_procs_def:
   network_procs NNil = []
 ∧ network_procs (NPar n1 n2) = network_procs n1 ++ network_procs n2
 ∧ network_procs (NEndpoint p s e) = [p]
-`;
+End
+
+val chor  = “c : chor”
+val pchor = “c : pchor”
 
 (* Projected networks identity over `network_procs` *)
-val network_procs_compile_id = Q.store_thm("network_procs_compile_id",
-  `∀s c l. network_procs (compile_network s c l) = l`,
+Theorem network_procs_chor_compile_id:
+  ∀s c l. network_procs (compile_network s ^chor l) = l
+Proof
   rw [] >> Induct_on `l`
-  \\ rw [network_procs_def,compile_network_gen_def]
-);
+  \\ rw [network_procs_def,
+         chor_to_endpointTheory.compile_network_gen_def]
+QED
+
+(* Projected networks identity over `network_procs` *)
+Theorem network_procs_pchor_compile_id:
+  ∀s c l. network_procs (compile_network s ^pchor l) = l
+Proof
+  rw [] >> Induct_on `l`
+  \\ rw [network_procs_def,
+         pchor_to_endpointTheory.compile_network_gen_def]
+QED
 
 (* Right End Point Network (`REPN`) is a network with only `NEndpoint` on the left
    and either `NNil` or other `REPN` on the right
@@ -29,15 +44,15 @@ val network_procs_compile_id = Q.store_thm("network_procs_compile_id",
                  |                  |                      |
                 NEndpoint p s e    NEndpoint p' s' e'     NNil
 *)
-val REPN_def = Define `
+Definition REPN_def:
   REPN NNil                        = T
 ∧ REPN (NEndpoint _ _ _)           = F
 ∧ REPN (NPar (NEndpoint _ _ _) ep) = REPN ep
 ∧ REPN _                           = F
-`;
+End
 
 (* A particular kind of congruence that only allows swaps to the right *)
-val (epn_rcong_rules, epn_rcong_ind, epn_rcong_cases) = Hol_reln `
+Inductive epn_rcong:
 (* Basic congruence rules *)
   (* Symmetric *)
   (∀c. epn_rcong c c)
@@ -59,7 +74,7 @@ val (epn_rcong_rules, epn_rcong_ind, epn_rcong_cases) = Hol_reln `
     epn_rcong n2 n2'
     ⇒ epn_rcong (NPar n1 n2)
                 (NPar n1 n2'))
-`;
+End
 
 val _ = Parse.add_infix("θ≅",425,Parse.NONASSOC);
 val _ = Parse.overload_on("θ≅",``epn_rcong``);
@@ -77,25 +92,56 @@ val epn_rcong_npair =  theorem "epn_rcong_pair";
 (* Two projected (using `compile_network`) networks are congruent as long as
    the list of projected process are permutable
 *)
-val PERM_rcong_compile_network = Q.store_thm("PERM_rcong_compile_network",
-  `∀l l' s c. PERM l l' ⇒ compile_network s c l θ≅ compile_network s c l'`,
+Theorem PERM_rcong_chor_compile_network:
+  ∀l l' s c. PERM l l'
+   ⇒ compile_network s ^chor l θ≅ compile_network s ^chor l'
+Proof
   rpt GEN_TAC
   \\ `∀l l'. PERM l l' ⇒ compile_network s c l θ≅ compile_network s c l'`
      suffices_by (metis_tac [])
   \\ ho_match_mp_tac PERM_IND
-  \\ rw [compile_network_gen_def,epn_rcong_rules]
+  \\ rw [chor_to_endpointTheory.compile_network_gen_def
+        ,epn_rcong_rules]
   >- (MAP_EVERY Q.ABBREV_TAC
-       [ `s1 = <|bindings := projectS x s; queue := []|>`
+       [ `s1 = <|bindings := chor_to_endpoint$projectS x s; queue := []|>`
        , `n1 = (project' x c)`
-       , `s2 = <|bindings := projectS y s; queue := []|>`
+       , `s2 = <|bindings := chor_to_endpoint$projectS y s; queue := []|>`
        , `n2 = (project' y c)`
-       , `n3 = compile_network s c l`
-       , `n4 = compile_network s c l'`]
+       , `n3 = compile_network s ^chor l`
+       , `n4 = compile_network s ^chor l'`]
      \\ ho_match_mp_tac epn_rcong_trans
      \\ Q.EXISTS_TAC `NPar (NEndpoint y s2 n2) (NPar (NEndpoint x s1 n1) n3)`
      \\ rw [epn_rcong_rules])
   >- (metis_tac [epn_rcong_trans])
-);
+QED
+
+(* Two projected (using `compile_network`) networks are congruent as long as
+   the list of projected process are permutable
+*)
+Theorem PERM_rcong_pchor_compile_network:
+  ∀l l' s c. PERM l l'
+   ⇒ compile_network s ^pchor l θ≅ compile_network s ^pchor l'
+Proof
+  rpt GEN_TAC
+  \\ `∀l l'. PERM l l' ⇒ compile_network s c l θ≅ compile_network s c l'`
+     suffices_by (metis_tac [])
+  \\ ho_match_mp_tac PERM_IND
+  \\ rw [pchor_to_endpointTheory.compile_network_gen_def
+        ,epn_rcong_rules]
+  >- (MAP_EVERY Q.ABBREV_TAC
+       [ `s1 = <|bindings := pchor_to_endpoint$projectS x s;
+                 queue    := projectQ' x [] c |>`
+       , `n1 = (project' x c)`
+       , `s2 = <|bindings := pchor_to_endpoint$projectS y s;
+                 queue    := projectQ' y [] c |>`
+       , `n2 = (project' y c)`
+       , `n3 = compile_network s ^pchor l`
+       , `n4 = compile_network s ^pchor l'`]
+     \\ ho_match_mp_tac epn_rcong_trans
+     \\ Q.EXISTS_TAC `NPar (NEndpoint y s2 n2) (NPar (NEndpoint x s1 n1) n3)`
+     \\ rw [epn_rcong_rules])
+  >- (metis_tac [epn_rcong_trans])
+QED
 
 (* If two (starting) networks (`n1`,`n1'`) are congruent then a
    transition with label `t` from any of them will imply there
@@ -110,11 +156,12 @@ val PERM_rcong_compile_network = Q.store_thm("PERM_rcong_compile_network",
   n1'------------------------------------n2'
 
 *)
-val epn_rcong_imp_trans = Q.store_thm("epn_rcong_imp_trans",
-  `∀n1 n1'.
+Theorem epn_rcong_imp_trans:
+   ∀n1 n1'.
     n1 θ≅ n1'
     ⇒ ∀t.(∀n2'. trans n1' t n2' ⇒ ∃n2.  trans n1  t n2  ∧ n2 θ≅ n2')
-       ∧ (∀n2.  trans n1  t n2  ⇒ ∃n2'. trans n1' t n2' ∧ n2' θ≅ n2)`,
+       ∧ (∀n2.  trans n1  t n2  ⇒ ∃n2'. trans n1' t n2' ∧ n2' θ≅ n2)
+Proof
   let val trans_metis = metis_tac [epn_rcong_rules,endpointSemTheory.trans_rules]
       val asm_epn_cases = (ASSUME_TAC o ONCE_REWRITE_RULE [endpointSemTheory.trans_cases])
       val epn_rcong_tac  =
@@ -141,23 +188,25 @@ val epn_rcong_imp_trans = Q.store_thm("epn_rcong_imp_trans",
   \\ TRY (qpat_x_assum `trans (NPar _ _) _ _` asm_epn_cases \\ rw [])
   \\ res_tac >> epn_tac
   end
-);
+QED
 
 (* A more human readable versin of `epn_rcong_imp_trans` *)
-val epn_rcong_trans' = Q.store_thm("epn_rcong_trans'",
-  `∀n1 n2 n1' t.
+Theorem epn_rcong_trans':
+   ∀n1 n2 n1' t.
     n1 θ≅ n1'
     ∧ trans n1 t n2
-    ⇒ ∃n2'. trans n1' t n2' ∧ n2 θ≅ n2'`,
+    ⇒ ∃n2'. trans n1' t n2' ∧ n2 θ≅ n2'
+Proof
   metis_tac [epn_rcong_imp_trans,epn_rcong_rules]
-);
+QED
 
 (* An extended RTC version of `epn_rcong_trans'` *)
-val epn_rcong_reduction = Q.store_thm("epn_rcong_reduction",
-  `∀n1 n2 n1'.
+Theorem epn_rcong_reduction:
+   ∀n1 n2 n1'.
     n1 θ≅ n1'
     ∧ reduction^* n1 n2
-    ⇒ ∃n2'. reduction^* n1' n2' ∧ n2 θ≅ n2'`,
+    ⇒ ∃n2'. reduction^* n1' n2' ∧ n2 θ≅ n2'
+Proof
   rpt GEN_TAC
   \\ `∀n1 n2. reduction^* n1 n2
        ⇒ ∀n1'. n1 θ≅ n1'
@@ -171,40 +220,52 @@ val epn_rcong_reduction = Q.store_thm("epn_rcong_reduction",
      \\ RES_TAC
      \\ fs [GSYM reduction_def]
      \\ metis_tac [RTC_RULES])
-);
+QED
 
 (* If a network is REPN and has no processes in it the is NNil *)
-val network_procs_NNil = Q.store_thm("network_procs_NNil",
-  `∀n. REPN n ∧ network_procs n = [] ⇒ n = NNil`,
+Theorem network_procs_NNil:
+  ∀n. REPN n ∧ network_procs n = [] ⇒ n = NNil
+Proof
   Induct_on `n`
   >- rw []
   >- (Cases_on `n`
      \\ Cases_on `n'`
      \\ rw [REPN_def,network_procs_def])
   >- rw [REPN_def,network_procs_def]
-);
+QED
 
 (* Projected networks are always REPN *)
-val REPN_compile_network = Q.store_thm("REPN_compile_network",
-  `∀s c l. REPN (compile_network s c l)`,
-  Induct_on `l` >> rw [REPN_def,compile_network_gen_def]
-);
+Theorem chor_REPN_compile_network:
+  ∀s c l. REPN (compile_network s ^chor l)
+Proof
+  Induct_on `l` >> rw [REPN_def,chor_to_endpointTheory.compile_network_gen_def]
+QED
+
+(* Projected networks are always REPN *)
+Theorem pchor_REPN_compile_network:
+  ∀s c l. REPN (compile_network s ^pchor l)
+Proof
+  Induct_on `l` >> rw [REPN_def,pchor_to_endpointTheory.compile_network_gen_def]
+QED
 
 (* Structural `REPN` reduction over `NPar` to the right *)
-val REPN_NPar = Q.store_thm("REPN_NPar",
-  `∀c c'. REPN (NPar c c') ⇒ REPN c'`,
+Theorem REPN_NPar:
+  ∀c c'. REPN (NPar c c') ⇒ REPN c'
+Proof
   Cases_on `c` >> rw [REPN_def]
-);
+QED
 
 (* Structural `REPN` reduction over `NPar` to the left *)
-val REPN_NPar_isNEndpoint = Q.store_thm("REPN_NPar_isNEndpoint",
-  `∀c c'. REPN (NPar c c') ⇒ ∃ p s e. c = NEndpoint p s e`,
+Theorem REPN_NPar_isNEndpoint:
+  ∀c c'. REPN (NPar c c') ⇒ ∃ p s e. c = NEndpoint p s e
+Proof
   Cases_on `c` >> rw [REPN_def]
-);
+QED
 
 (* endpoint network congruence preserves `REPN` *)
-val rcong_REPN = Q.store_thm("rcong_REPN",
-  `∀c c'. c θ≅ c' ⇒ (REPN c ⇔ REPN c')`,
+Theorem rcong_REPN:
+  ∀c c'. c θ≅ c' ⇒ (REPN c ⇔ REPN c')
+Proof
   ho_match_mp_tac epn_rcong_ind
   \\ rw []
   >- (EQ_TAC
@@ -214,47 +275,51 @@ val rcong_REPN = Q.store_thm("rcong_REPN",
      \\ IMP_RES_TAC REPN_NPar_isNEndpoint
      \\ rw [REPN_def])
   >- (Cases_on `n1` \\ rw [REPN_def])
-);
+QED
 
 (* endpoint network congruence preserves all t
    he contents (endpoints) of the network
 *)
-val rcong_PERM_enpoints = Q.store_thm("rcong_PERM_enpoints",
-  `∀ep ep'. ep θ≅ ep' ⇒ PERM (endpoints ep) (endpoints ep')`,
+Theorem rcong_PERM_enpoints:
+  ∀ep ep'. ep θ≅ ep' ⇒ PERM (endpoints ep) (endpoints ep')
+Proof
   ho_match_mp_tac epn_rcong_ind
   \\ rw []
   >- metis_tac [PERM_SYM,PERM_TRANS]
   >- metis_tac [PERM_SYM,PERM_TRANS]
   >- rw [endpoints_def,PERM_SWAP_L_AT_FRONT]
   >- rw [endpoints_def,PERM_APPEND_IFF]
-);
+QED
 
 (* `epnList` constructs a network from a list of endpoints (as pairs) *)
-val epnList_def = Define`
+Definition epnList_def:
   epnList [] = NNil
 ∧ epnList ((p,s,e)::l) = NPar (NEndpoint p s e) (epnList l)
-`;
+End
 
 (* `epnList` networks are always REPN *)
-val epnList_REPN = Q.store_thm("epnList_REPN",
-  `∀l. REPN (epnList l)`,
+Theorem epnList_REPN:
+  ∀l. REPN (epnList l)
+Proof
   Induct_on `l` \\ rw [REPN_def,epnList_def]
   \\ Cases_on `h` \\ Cases_on `r` \\ rw [REPN_def,epnList_def]
-);
+QED
 
 (* `epnList o endpoints = id` *)
-val epnList_id = Q.store_thm("epnList_id",
-  `∀l. l = endpoints (epnList l)`,
+Theorem epnList_id:
+  ∀l. l = endpoints (epnList l)
+Proof
   Induct_on `l` \\ rw [endpoints_def,epnList_def]
   \\ Cases_on `h` \\ Cases_on `r` \\ rw [endpoints_def,epnList_def]
-);
+QED
 
 (* IF two REPN networks have the same contents THEN they are congruent *)
-val REPN_PERM_rcong = Q.store_thm("REPN_PERM_rcong",
-  `∀ep ep'.
+Theorem REPN_PERM_rcong:
+   ∀ep ep'.
     PERM (endpoints ep) (endpoints ep')
     ∧ REPN ep ∧ REPN ep'
-    ⇒ ep θ≅ ep'`,
+    ⇒ ep θ≅ ep'
+Proof
   rpt GEN_TAC
   \\ `∀l l'. PERM l l'
        ⇒ ∀ep ep'. l = endpoints ep
@@ -286,16 +351,17 @@ val REPN_PERM_rcong = Q.store_thm("REPN_PERM_rcong",
         \\ RES_TAC
         \\ metis_tac [epn_rcong_trans])
      end
-);
+QED
 
 (* IF two REPN networks are congruent and have the same left side,
    their right side must be congruent
 *)
-val epn_rcong_NPar = Q.store_thm("epn_rcong_NPar",
-  `∀n1 n2 n3. NPar n1 n2 θ≅ NPar n1 n3
+Theorem epn_rcong_NPar:
+   ∀n1 n2 n3. NPar n1 n2 θ≅ NPar n1 n3
     ∧ REPN (NPar n1 n2)
     ∧ REPN (NPar n1 n3)
-    ⇒ n2 θ≅ n3`,
+    ⇒ n2 θ≅ n3
+Proof
    rw []
    \\ IMP_RES_TAC REPN_NPar_isNEndpoint
    \\ fs []
@@ -304,64 +370,119 @@ val epn_rcong_NPar = Q.store_thm("epn_rcong_NPar",
    \\ fs [endpoints_def]
    \\ IMP_RES_TAC REPN_NPar
    \\ IMP_RES_TAC REPN_PERM_rcong
-);
+QED
 
 (* Every element in a projected choreography is a projection of
    state and endpoint for an specific process
 
    PS: this is obvious, but it's convenient to have
 *)
-val compile_network_MEM_elem = Q.store_thm("compile_network_MEM_elem",
-  `∀p s e c s' l.
-    MEM (p,s',e) (endpoints (compile_network s c l))
-    ⇒ s' = <|bindings := projectS p s; queue := []|>
-      ∧ e = project' p c`,
+Theorem chor_compile_network_MEM_elem:
+   ∀p s e c s' l.
+    MEM (p,s',e) (endpoints (compile_network s ^chor l))
+    ⇒ s' = <|bindings := chor_to_endpoint$projectS p s; queue := []|>
+      ∧ e = project' p ^chor
+Proof
   rpt GEN_TAC
   \\ Induct_on `l`
-  \\ rw [MEM,compile_network_gen_def,endpoints_def]
+  \\ rw [MEM,chor_to_endpointTheory.compile_network_gen_def,endpoints_def]
   \\ fs []
-);
+QED
+
+(* Every element in a projected partial choreography is a projection
+   of state and endpoint for an specific process
+
+   PS: this is obvious, but it's convenient to have
+ *)
+Theorem pchor_compile_network_MEM_elem:
+   ∀p s e c s' l.
+    MEM (p,s',e) (endpoints (compile_network s ^pchor l))
+    ⇒ s' = <|bindings := pchor_to_endpoint$projectS p s;
+             queue    := projectQ' p [] ^pchor |>
+      ∧ e = project' p ^pchor
+Proof
+  rpt GEN_TAC
+  \\ Induct_on `l`
+  \\ rw [MEM,pchor_to_endpointTheory.compile_network_gen_def,endpoints_def]
+  \\ fs []
+QED
 
 (* One can pull (using congruence) any element of a projected network
    to be the top-most endpoint
 *)
-val compile_network_pull = Q.store_thm("compile_network_pull",
-  `∀p s e s' c l ep.
+Theorem chor_compile_network_pull:
+   ∀p s e s' c l ep.
     ALL_DISTINCT l
-    ∧ MEM (p,s,e) (endpoints (compile_network s' c l))
-    ∧ ep = compile_network s' c (FILTER ($≠ p) l)
-    ⇒ compile_network s' c l θ≅ NPar (NEndpoint p s e) ep`,
+    ∧ MEM (p,s,e) (endpoints (compile_network s' ^chor l))
+    ∧ ep = compile_network s' ^chor (FILTER ($≠ p) l)
+    ⇒ compile_network s' ^chor l θ≅ NPar (NEndpoint p s e) ep
+Proof
   rw []
   \\ Induct_on `l` \\ rw []
-  >- fs [compile_network_gen_def,endpoints_def,MEM]
-  >- (fs [compile_network_gen_def,endpoints_def,MEM] \\ fs []
-     \\ Q.ABBREV_TAC `h_ep = NEndpoint h <|bindings := projectS h s'; queue := []|> (project' h c)`
+  >- fs [chor_to_endpointTheory.compile_network_gen_def,endpoints_def,MEM]
+  >- (fs [chor_to_endpointTheory.compile_network_gen_def,endpoints_def,MEM] \\ fs []
+     \\ Q.ABBREV_TAC `h_ep =
+           NEndpoint h <| bindings := chor_to_endpoint$projectS h s';
+                          queue    := [] |> (project' h ^chor)`
      \\ ho_match_mp_tac epn_rcong_trans
      \\ Q.EXISTS_TAC `NPar h_ep
                            (NPar (NEndpoint p s e)
-                           (compile_network s' c (FILTER (λy. p ≠ y) l)))`
+                           (compile_network s' ^chor (FILTER (λy. p ≠ y) l)))`
      \\ rw [Abbr `h_ep`, epn_rcong_swap]
      \\ ho_match_mp_tac epn_rcong_npair
      \\ rw [])
-  >- (fs [compile_network_gen_def,endpoints_def,MEM] \\ fs []
+  >- (fs [chor_to_endpointTheory.compile_network_gen_def,endpoints_def,MEM] \\ fs []
      \\ `¬MEM h l ⇒ FILTER ($≠ h) l = l`
         by (rpt (pop_assum (K ALL_TAC))
            \\ Induct_on `l`
            \\ rw [MEM_FILTER,FILTER])
-     \\ metis_tac [epn_rcong_refl,compile_network_MEM_elem])
-);
+     \\ metis_tac [epn_rcong_refl,chor_compile_network_MEM_elem])
+QED
+
+(* One can pull (using congruence) any element of a projected network
+   to be the top-most endpoint
+*)
+Theorem pchor_compile_network_pull:
+   ∀p s e s' c l ep.
+    ALL_DISTINCT l
+    ∧ MEM (p,s,e) (endpoints (compile_network s' ^pchor l))
+    ∧ ep = compile_network s' ^pchor (FILTER ($≠ p) l)
+    ⇒ compile_network s' ^pchor l θ≅ NPar (NEndpoint p s e) ep
+Proof
+  rw []
+  \\ Induct_on `l` \\ rw []
+  >- fs [pchor_to_endpointTheory.compile_network_gen_def,endpoints_def,MEM]
+  >- (fs [pchor_to_endpointTheory.compile_network_gen_def,endpoints_def,MEM] \\ fs []
+     \\ Q.ABBREV_TAC `h_ep =
+           NEndpoint h <| bindings := pchor_to_endpoint$projectS h s';
+                          queue    := projectQ' h [] c |> (project' h ^pchor)`
+     \\ ho_match_mp_tac epn_rcong_trans
+     \\ Q.EXISTS_TAC `NPar h_ep
+                           (NPar (NEndpoint p s e)
+                           (compile_network s' ^pchor (FILTER (λy. p ≠ y) l)))`
+     \\ rw [Abbr `h_ep`, epn_rcong_swap]
+     \\ ho_match_mp_tac epn_rcong_npair
+     \\ rw [])
+  >- (fs [pchor_to_endpointTheory.compile_network_gen_def,endpoints_def,MEM] \\ fs []
+     \\ `¬MEM h l ⇒ FILTER ($≠ h) l = l`
+        by (rpt (pop_assum (K ALL_TAC))
+           \\ Induct_on `l`
+           \\ rw [MEM_FILTER,FILTER])
+     \\ metis_tac [epn_rcong_refl,pchor_compile_network_MEM_elem])
+QED
 
 (* Any network that is congruent with a projected network, can be
    expressed as a projection (using `compile_network`)
 *)
-val compile_network_rcong = Q.store_thm("compile_network_rcong",
-  `∀s c l ep. compile_network s c l θ≅ ep ∧ ALL_DISTINCT l
-    ⇒ ep = compile_network s c (network_procs ep)`,
+Theorem chor_compile_network_rcong:
+   ∀s c l ep. compile_network s ^chor l θ≅ ep ∧ ALL_DISTINCT l
+    ⇒ ep = compile_network s ^chor (network_procs ep)
+Proof
   Induct_on `ep`
-  >- (rw [compile_network_gen_def,network_procs_def])
+  >- (rw [chor_to_endpointTheory.compile_network_gen_def,network_procs_def])
   >- (rw []
-     \\ `REPN (compile_network s c l)`
-        by rw [REPN_compile_network]
+     \\ `REPN (compile_network s ^chor l)`
+        by rw [chor_REPN_compile_network]
      \\ IMP_RES_TAC rcong_REPN
      \\ IMP_RES_TAC REPN_NPar_isNEndpoint
      \\ rw []
@@ -372,34 +493,75 @@ val compile_network_rcong = Q.store_thm("compile_network_rcong",
          by metis_tac [PERM_MEM_EQ]
      \\ Q.ABBREV_TAC `l' = compile_network s c (FILTER ($≠ p) l)`
      \\ `NPar (NEndpoint p s' e) l' θ≅ compile_network s c l`
-        by (rw [Abbr `l'`] >> metis_tac [compile_network_pull,epn_rcong_sym])
+        by (rw [Abbr `l'`] >> metis_tac [chor_compile_network_pull,epn_rcong_sym])
      \\ `NPar (NEndpoint p s' e) l' θ≅ NPar (NEndpoint p s' e) ep'`
         by (rw [Abbr `l'`] >> metis_tac [epn_rcong_trans])
      \\ `l' θ≅ ep'`
         by (rw [Abbr `l'`] >> metis_tac [epn_rcong_NPar,rcong_REPN])
-     \\ rw [compile_network_gen_def,network_procs_def,compile_network_MEM_elem]
-     \\ IMP_RES_TAC compile_network_MEM_elem
+     \\ rw [chor_to_endpointTheory.compile_network_gen_def,network_procs_def,
+            chor_compile_network_MEM_elem]
+     \\ IMP_RES_TAC chor_compile_network_MEM_elem
      \\ UNABBREV_ALL_TAC
      \\ metis_tac [FILTER_ALL_DISTINCT])
  >- (rw []
-    \\ `REPN (compile_network s' c l')` by rw [REPN_compile_network]
+    \\ `REPN (compile_network s' c l')` by rw [chor_REPN_compile_network]
     \\ IMP_RES_TAC rcong_REPN
     \\ fs [REPN_def])
-);
+QED
+
+(* Any network that is congruent with a projected network, can be
+   expressed as a projection (using `compile_network`)
+*)
+Theorem pchor_compile_network_rcong:
+   ∀s c l ep. compile_network s ^pchor l θ≅ ep ∧ ALL_DISTINCT l
+    ⇒ ep = compile_network s ^pchor (network_procs ep)
+Proof
+  Induct_on `ep`
+  >- (rw [pchor_to_endpointTheory.compile_network_gen_def,network_procs_def])
+  >- (rw []
+     \\ `REPN (compile_network s ^pchor l)`
+        by rw [pchor_REPN_compile_network]
+     \\ IMP_RES_TAC rcong_REPN
+     \\ IMP_RES_TAC REPN_NPar_isNEndpoint
+     \\ rw []
+     \\ IMP_RES_TAC rcong_PERM_enpoints
+     \\ `MEM (p,s',e) (endpoints (NPar (NEndpoint p s' e) ep'))`
+        by rw [endpoints_def]
+     \\ `MEM (p,s',e) (endpoints (compile_network s c l))`
+         by metis_tac [PERM_MEM_EQ]
+     \\ Q.ABBREV_TAC `l' = compile_network s c (FILTER ($≠ p) l)`
+     \\ `NPar (NEndpoint p s' e) l' θ≅ compile_network s c l`
+        by (rw [Abbr `l'`] >> metis_tac [pchor_compile_network_pull,epn_rcong_sym])
+     \\ `NPar (NEndpoint p s' e) l' θ≅ NPar (NEndpoint p s' e) ep'`
+        by (rw [Abbr `l'`] >> metis_tac [epn_rcong_trans])
+     \\ `l' θ≅ ep'`
+        by (rw [Abbr `l'`] >> metis_tac [epn_rcong_NPar,rcong_REPN])
+     \\ rw [pchor_to_endpointTheory.compile_network_gen_def,network_procs_def,
+            pchor_compile_network_MEM_elem]
+     \\ IMP_RES_TAC pchor_compile_network_MEM_elem
+     \\ UNABBREV_ALL_TAC
+     \\ metis_tac [FILTER_ALL_DISTINCT])
+ >- (rw []
+    \\ `REPN (compile_network s' c l')` by rw [pchor_REPN_compile_network]
+    \\ IMP_RES_TAC rcong_REPN
+    \\ fs [REPN_def])
+QED
 
 (* Networks preserve the number of process over transitions *)
-val network_procs_trans = Q.store_thm("network_procs_trans",
-  `∀ep t ep'. trans ep t ep' ⇒ network_procs ep' = network_procs ep`,
+Theorem network_procs_trans:
+  ∀ep t ep'. trans ep t ep' ⇒ network_procs ep' = network_procs ep
+Proof
   ho_match_mp_tac endpointSemTheory.trans_ind
   \\ rw [network_procs_def]
-);
+QED
 
-val network_procs_reduction = Q.store_thm("network_procs_reduction",
-  `∀ep ep'. reduction^* ep ep' ⇒ network_procs ep' = network_procs ep`,
+Theorem network_procs_reduction:
+  ∀ep ep'. reduction^* ep ep' ⇒ network_procs ep' = network_procs ep
+Proof
   ho_match_mp_tac RTC_INDUCT
   \\ rw [reduction_def]
   \\ IMP_RES_TAC network_procs_trans
-);
+QED
 
 (* A transitions between projected networks with list of process `l1`
    implies the same transition can be made between projected networks
@@ -419,94 +581,191 @@ val network_procs_reduction = Q.store_thm("network_procs_reduction",
       `trans (compile_network s c l1) t (compile_network s c' l1)`
       however I'm including it for completeness
 *)
-val PERM_compile_network_trans = Q.store_thm("PERM_compile_network_trans",
-  `∀s c c' t l1 l2.
+Theorem chor_PERM_compile_network_trans:
+   ∀s c (c' : chor) t l1 l2.
     PERM l1 l2
     ∧ ALL_DISTINCT l1
-    ∧ trans (compile_network s c l1) t (compile_network s c' l1)
-    ⇒ trans (compile_network s c l2) t (compile_network s c' l2)`,
+    ∧ trans (compile_network s ^chor l1) t (compile_network s c' l1)
+    ⇒ trans (compile_network s ^chor l2) t (compile_network s c' l2)
+Proof
     rw []
     \\ `compile_network s c l1 θ≅ compile_network s c l2`
-       by rw [PERM_rcong_compile_network]
+       by rw [PERM_rcong_chor_compile_network]
     \\ IMP_RES_TAC epn_rcong_trans'
     \\ IMP_RES_TAC network_procs_trans
-    \\ IMP_RES_TAC compile_network_rcong
-    \\ rfs [network_procs_compile_id]
+    \\ IMP_RES_TAC chor_compile_network_rcong
+    \\ rfs [network_procs_chor_compile_id]
     \\ rw []
-);
+QED
 
-
-(* An RTC variant of `PERM_compile_network_trans`, way more relevant and useful *)
-val PERM_compile_network_reduction = Q.store_thm("PERM_compile_network_reduction",
-  `∀s c c' l1 l2.
+(* See ‘chor_PERM_compile_network_trans’ (above) for a nice explanation *)
+Theorem pchor_PERM_compile_network_trans:
+   ∀s c (c' : pchor) t l1 l2.
     PERM l1 l2
     ∧ ALL_DISTINCT l1
-    ∧ reduction^* (compile_network s c l1) (compile_network s c' l1)
-    ⇒ reduction^* (compile_network s c l2) (compile_network s c' l2)`,
+    ∧ trans (compile_network s ^pchor l1) t (compile_network s c' l1)
+    ⇒ trans (compile_network s ^pchor l2) t (compile_network s c' l2)
+Proof
     rw []
     \\ `compile_network s c l1 θ≅ compile_network s c l2`
-       by rw [PERM_rcong_compile_network]
+       by rw [PERM_rcong_pchor_compile_network]
+    \\ IMP_RES_TAC epn_rcong_trans'
+    \\ IMP_RES_TAC network_procs_trans
+    \\ IMP_RES_TAC pchor_compile_network_rcong
+    \\ rfs [network_procs_pchor_compile_id]
+    \\ rw []
+QED
+
+(* An RTC variant of `PERM_chor_compile_network_trans`, way more relevant and useful *)
+Theorem PERM_chor_compile_network_reduction:
+   ∀s c (c' : chor) l1 l2.
+    PERM l1 l2
+    ∧ ALL_DISTINCT l1
+    ∧ reduction^* (compile_network s ^chor l1) (compile_network s c' l1)
+    ⇒ reduction^* (compile_network s ^chor l2) (compile_network s c' l2)
+Proof
+    rw []
+    \\ `compile_network s c l1 θ≅ compile_network s c l2`
+       by rw [PERM_rcong_chor_compile_network]
     \\ IMP_RES_TAC epn_rcong_reduction
     \\ IMP_RES_TAC network_procs_reduction
-    \\ IMP_RES_TAC compile_network_rcong
-    \\ rfs [network_procs_compile_id]
+    \\ IMP_RES_TAC chor_compile_network_rcong
+    \\ rfs [network_procs_chor_compile_id]
     \\ rw []
-);
+QED
 
-(* `Com` instance of `PERM_compile_network_reduction` with more
+(* An RTC variant of `PERM_pchor_compile_network_trans`, way more relevant and useful *)
+Theorem PERM_pchor_compile_network_reduction:
+   ∀s c (c' : pchor) l1 l2.
+    PERM l1 l2
+    ∧ ALL_DISTINCT l1
+    ∧ reduction^* (compile_network s ^pchor l1) (compile_network s c' l1)
+    ⇒ reduction^* (compile_network s ^pchor l2) (compile_network s c' l2)
+Proof
+    rw []
+    \\ `compile_network s c l1 θ≅ compile_network s c l2`
+       by rw [PERM_rcong_pchor_compile_network]
+    \\ IMP_RES_TAC epn_rcong_reduction
+    \\ IMP_RES_TAC network_procs_reduction
+    \\ IMP_RES_TAC pchor_compile_network_rcong
+    \\ rfs [network_procs_pchor_compile_id]
+    \\ rw []
+QED
+
+(* `Com` instance of `PERM_chor_compile_network_reduction` with more
    specific assumptions
 *)
-val compile_network_COM = Q.store_thm("compile_network_COM",
- `∀s c p x q y l.
+Theorem chor_compile_network_COM:
+  ∀s ^chor p x q y l.
    PERM (procsOf (Com  p x q y c)) l
    ∧ p ≠ q
    ∧ reduction^* (compile_network s (Com  p x q y c) (p::q::FILTER (λx. p ≠ x ∧ q ≠ x) l))
                  (compile_network s               c  (p::q::FILTER (λx. p ≠ x ∧ q ≠ x) l))
-   ⇒ reduction^* (compile_network s (Com  p x q y c) l) (compile_network s c l)`,
+   ⇒ reduction^* (compile_network s (Com  p x q y c) l) (compile_network s c l)
+Proof
     rw []
     \\ Q.ABBREV_TAC `l' = p::q::FILTER (λx. p ≠ x ∧ q ≠ x) l`
     \\ `ALL_DISTINCT l`
-       by metis_tac [ALL_DISTINCT_PERM,procsOf_all_distinct]
+       by metis_tac [ALL_DISTINCT_PERM,chorSemTheory.procsOf_all_distinct]
     \\ `ALL_DISTINCT l'`
        by rw [Abbr `l'`,ALL_DISTINCT,MEM_FILTER,FILTER_ALL_DISTINCT]
     \\ `MEM p l ∧ MEM q l`
        by (`MEM p (procsOf (Com  p x q y c)) ∧ MEM q (procsOf (Com  p x q y c))`
-          by rw [MEM,procsOf_def,nub'_def]
+          by rw [MEM,chorSemTheory.procsOf_def,chorSemTheory.nub'_def]
           \\ metis_tac [MEM_PERM])
     \\ `PERM l' l`
        by (ho_match_mp_tac PERM_ALL_DISTINCT
           \\ rw [Abbr `l'`]
           \\ Cases_on `p ≠ x'` \\ Cases_on `q ≠ x'`
           \\ rw [MEM_FILTER])
-    \\ metis_tac [PERM_compile_network_reduction]
-);
+    \\ metis_tac [PERM_chor_compile_network_reduction]
+QED
 
-(* `Sel` instance of `PERM_compile_network_reduction` with more
+(* `Com` instance of `PERM_pchor_compile_network_reduction` with more
    specific assumptions
 *)
-val compile_network_SEL = Q.store_thm("compile_network_SEL",
- `∀s c p b q l.
+Theorem pchor_compile_network_COM:
+  ∀s ^pchor p x q y l.
+   PERM (procsOf (Com  p x q y c)) l
+   ∧ p ≠ q
+   ∧ reduction^* (compile_network s (Com  p x q y c) (p::q::FILTER (λx. p ≠ x ∧ q ≠ x) l))
+                 (compile_network s               c  (p::q::FILTER (λx. p ≠ x ∧ q ≠ x) l))
+   ⇒ reduction^* (compile_network s (Com  p x q y c) l) (compile_network s c l)
+Proof
+    rw []
+    \\ Q.ABBREV_TAC `l' = p::q::FILTER (λx. p ≠ x ∧ q ≠ x) l`
+    \\ `ALL_DISTINCT l`
+       by metis_tac [ALL_DISTINCT_PERM,pchorSemTheory.procsOf_all_distinct]
+    \\ `ALL_DISTINCT l'`
+       by rw [Abbr `l'`,ALL_DISTINCT,MEM_FILTER,FILTER_ALL_DISTINCT]
+    \\ `MEM p l ∧ MEM q l`
+       by (`MEM p (procsOf (Com  p x q y c)) ∧ MEM q (procsOf (Com  p x q y c))`
+          by rw [MEM,pchorSemTheory.procsOf_def,nub_def]
+          \\ metis_tac [MEM_PERM])
+    \\ `PERM l' l`
+       by (ho_match_mp_tac PERM_ALL_DISTINCT
+          \\ rw [Abbr `l'`]
+          \\ Cases_on `p ≠ x'` \\ Cases_on `q ≠ x'`
+          \\ rw [MEM_FILTER])
+    \\ metis_tac [PERM_pchor_compile_network_reduction]
+QED
+
+(* `Sel` instance of `PERM_chor_compile_network_reduction` with more
+   specific assumptions
+*)
+Theorem chor_compile_network_SEL:
+  ∀s ^chor p b q l.
    PERM (procsOf (Sel  p b q c)) l
    ∧ p ≠ q
    ∧ reduction^* (compile_network s (Sel p b q c) (p::q::FILTER (λx. p ≠ x ∧ q ≠ x) l))
                  (compile_network s            c  (p::q::FILTER (λx. p ≠ x ∧ q ≠ x) l))
-   ⇒ reduction^* (compile_network s (Sel p b q c) l) (compile_network s c l)`,
+   ⇒ reduction^* (compile_network s (Sel p b q c) l) (compile_network s c l)
+Proof
     rw []
     \\ Q.ABBREV_TAC `l' = p::q::FILTER (λx. p ≠ x ∧ q ≠ x) l`
     \\ `ALL_DISTINCT l`
-       by metis_tac [ALL_DISTINCT_PERM,procsOf_all_distinct]
+       by metis_tac [ALL_DISTINCT_PERM,chorSemTheory.procsOf_all_distinct]
     \\ `ALL_DISTINCT l'`
        by rw [Abbr `l'`,ALL_DISTINCT,MEM_FILTER,FILTER_ALL_DISTINCT]
     \\ `MEM p l ∧ MEM q l`
        by (`MEM p (procsOf (Sel  p b q c)) ∧ MEM q (procsOf (Sel p b q c))`
-          by rw [MEM,procsOf_def,nub'_def]
+          by rw [MEM,chorSemTheory.procsOf_def,chorSemTheory.nub'_def]
           \\ metis_tac [MEM_PERM])
     \\ `PERM l' l`
        by (ho_match_mp_tac PERM_ALL_DISTINCT
           \\ rw [Abbr `l'`]
           \\ Cases_on `p ≠ x` \\ Cases_on `q ≠ x`
           \\ rw [MEM_FILTER])
-    \\ metis_tac [PERM_compile_network_reduction]
-);
+    \\ metis_tac [PERM_chor_compile_network_reduction]
+QED
+
+(* `Sel` instance of `PERM_pchor_compile_network_reduction` with more
+   specific assumptions
+*)
+Theorem pchor_compile_network_SEL:
+  ∀s ^pchor p b q l.
+   PERM (procsOf (Sel  p b q c)) l
+   ∧ p ≠ q
+   ∧ reduction^* (compile_network s (Sel p b q c) (p::q::FILTER (λx. p ≠ x ∧ q ≠ x) l))
+                 (compile_network s            c  (p::q::FILTER (λx. p ≠ x ∧ q ≠ x) l))
+   ⇒ reduction^* (compile_network s (Sel p b q c) l) (compile_network s c l)
+Proof
+    rw []
+    \\ Q.ABBREV_TAC `l' = p::q::FILTER (λx. p ≠ x ∧ q ≠ x) l`
+    \\ `ALL_DISTINCT l`
+       by metis_tac [ALL_DISTINCT_PERM,pchorSemTheory.procsOf_all_distinct]
+    \\ `ALL_DISTINCT l'`
+       by rw [Abbr `l'`,ALL_DISTINCT,MEM_FILTER,FILTER_ALL_DISTINCT]
+    \\ `MEM p l ∧ MEM q l`
+       by (`MEM p (procsOf (Sel  p b q c)) ∧ MEM q (procsOf (Sel p b q c))`
+          by rw [MEM,pchorSemTheory.procsOf_def,nub_def]
+          \\ metis_tac [MEM_PERM])
+    \\ `PERM l' l`
+       by (ho_match_mp_tac PERM_ALL_DISTINCT
+          \\ rw [Abbr `l'`]
+          \\ Cases_on `p ≠ x` \\ Cases_on `q ≠ x`
+          \\ rw [MEM_FILTER])
+    \\ metis_tac [PERM_pchor_compile_network_reduction]
+QED
 
 val _ = export_theory ()
