projection/pchor_to_endpointScript.sml
@@ -275,6 +275,10 @@ val _ = overload_on("compile_network_ok",
   ``(λs c l. FST (compile_network_gen s c l))``
 );
 
+val _ = overload_on("projectQ'",
+  ``(λp l c. SND (projectQ p l c))``
+);
+
 val _ = overload_on("project'",
   ``(λp c. SND (project p c))``
 );
